eve/Src/framework/eve_proofs/writer/ep_frame_extractor.e
@@ -1,0 +1,86 @@
+indexing
+	description:
+		"[
+			TODO
+		]"
+	date: "$Date$"
+	revision: "$Revision$"
+
+class EP_FRAME_EXTRACTOR
+
+inherit
+
+	EP_VISITOR
+
+	SHARED_EP_ENVIRONMENT
+		export {NONE} all end
+
+create
+	make
+
+feature {NONE} -- Initialization
+
+	make
+			-- Initialize frame extractor.
+		do
+			create last_frame_condition.make_empty
+		end
+
+feature -- Access
+
+	last_frame_condition: STRING
+			-- Last built frame condition
+
+feature -- Basic operations
+
+	build_frame_condition (a_feature: !FEATURE_I)
+			-- Build frame condition for feature `a_feature'.
+		do
+			if is_pure (a_feature) then
+				last_frame_condition := "frame.modifies_nothing(Heap, old(Heap))"
+			else
+				last_frame_condition := "true"
+			end
+		ensure
+			frame_condition_built: not last_frame_condition.is_empty
+		end
+
+feature {NONE} -- Visitors
+
+
+feature {NONE} -- Implementation
+
+
+-- TODO: move someplace else and improve
+	is_pure (a_feature: !FEATURE_I): BOOLEAN
+			-- Is `a_feature' a pure feature?
+		local
+			l_indexing_clause: INDEXING_CLAUSE_AS
+			l_index: INDEX_AS
+			l_bool: BOOL_AS
+			l_found: BOOLEAN
+		do
+			Result := feature_list.features_used_in_contracts.has (a_feature)
+			if not Result then
+				l_indexing_clause := a_feature.written_class.ast.feature_with_name (a_feature.feature_name_id).indexes
+				if l_indexing_clause /= Void then
+					from
+						l_indexing_clause.start
+					until
+						l_indexing_clause.after or l_found
+					loop
+						l_index := l_indexing_clause.item
+						if l_index.tag.name.as_lower.is_equal ("pure") then
+							l_found := True
+							l_bool ?= l_index.index_list.first
+							if l_bool /= Void then
+								Result := l_bool.value
+							end
+						end
+						l_indexing_clause.forth
+					end
+				end
+			end
+		end
+
+end
